\documentclass[10pt,english]{article}
\usepackage[T1]{fontenc}
\usepackage[latin9]{inputenc}
\usepackage{geometry}
\geometry{verbose,tmargin=1.5in,bmargin=1.5in,lmargin=1.5in,rmargin=1.5in}
\usepackage{amsthm}
\usepackage{amsmath}
\usepackage{amssymb}

\makeatletter
\usepackage{enumitem}
\newlength{\lyxlabelwidth}

\usepackage[T1]{fontenc}
\usepackage{ae,aecompl}

%\usepackage{txfonts}

\usepackage{microtype}

\usepackage{calc}
\usepackage{enumitem}
\setenumerate{leftmargin=!,labelindent=0pt,itemindent=0em,labelwidth=\widthof{\ref{last-item}}}

\makeatother

\usepackage{babel}
\begin{document}
\noindent \begin{center}
\textbf{\large{}MATH 146 - Assignment 2}\\
\textbf{\large{}Chris Ji 20725415}
\par\end{center}{\large \par}
\medskip{}

\begin{enumerate}
\item \begin{enumerate}
    \item [a)] Let $B=\begin{bmatrix}b_{11} & b_{12}\\b_{21} & b_{22}\end{bmatrix}$. Then $AB=\begin{bmatrix}b_{11} & b_{12}\\b_{11}+b_{21} & b_{12}+b_{22}\end{bmatrix}$, and $BA = \begin{bmatrix}b_{11}+b_{12} & b_{12}\\b_{21}+b_{22} & b_{22}\end{bmatrix}$. For $AB$ to be equal to $BA$, $b_{12}$ must equal $0$ for $(AB)_{11}=(BA)_{11}$ and $(AB)_{22}=(BA)_{22}$. Furthermore, $b_{11}=b_{22}$ for $(AB)_{21}=(BA)_{21}$. 
    \item [b)] Let $A=\begin{bmatrix}a_{11} & a_{12}\\a_{21} & a_{22}\end{bmatrix}$ and $B$ from above, $AB=\begin{bmatrix}a_{11}b_{11}+a_{12}b_{21} & a_{11}b_{12}+a_{12}b_{22}\\a_{21}b_{11}+a_{22}b_{21} & a_{21}b_{12}+a_{22}b_{22}\end{bmatrix}$ and $BA=\begin{bmatrix}b_{11}a_{11}+b_{12}a_{21} & b_{11}a_{12}+b_{12}a_{22}\\b_{21}a_{11}+b_{22}a_{21} & b_{21}a_{12}+b_{22}a_{22}\end{bmatrix}$. $(AB-BA)=\begin{bmatrix}a_{12}b_{21}-a_{21}b_{12} & a_{11}b_{12}+a_{12}b_{22}-a_{12}b_{11}-a_{22}b_{12}\\a_{21}b_{11}+a_{22}b_{21}-a_{11}b_{21}-a_{21}b_{22} & a_{21}b_{12}-a_{12}b_{21}\end{bmatrix}$. 
\end{enumerate}

\item \begin{enumerate}
    \item [a)]
    \item [b)]
\end{enumerate}

\item 

\item \begin{enumerate}
    \item [a)]
    \item [b)]
\end{enumerate}

\item \begin{enumerate}
    \item [a)]
    \item [b)]
    \item [c)]
    \item [d)]
\end{enumerate}
\end{enumerate}

\end{document}
